@prefix owl: <http://www.w3.org/2002/07/owl#> .
@prefix rdf: <http://www.w3.org/1999/02/22-rdf-syntax-ns#> .
@prefix sco: <https://www.bim-sis.de/ontology/damage/sco#> .
@prefix xml: <http://www.w3.org/XML/1998/namespace> .
@prefix xsd: <http://www.w3.org/2001/XMLSchema#> .
@prefix foaf: <http://xmlns.com/foaf/0.1/> .
@prefix rdfs: <http://www.w3.org/2000/01/rdf-schema#> .
@prefix cto: <https://w3id.org/cto#> .
@prefix srmo: <https://w3id.org/srmo#> .
@prefix vann: <http://purl.org/vocab/vann/> .
@prefix voaf: <http://purl.org/vocommons/voaf#> .
@prefix dcterms: <http://purl.org/dc/terms/> .

<https://www.bim-sis.de/ontology/damage/srmo> rdf:type owl:Ontology ;
                                              owl:versionIRI <https://www.bim-sis.de/ontology/damage/srmo/0.1> ;
                                              dcterms:creator [ rdf:type foaf:Person ;
                                                                 foaf:name "Al-Hakam Hamdan"
                                                               ] ,
                                                               [ rdf:type foaf:Person ;
                                                                 foaf:name "Peter Katranuschkov"
                                                               ] ;
dcterms:description "Ontology that defines renovation measures applied for stone maintenance."@en ;
dcterms:issued "2021-01-13"^^xsd:date ;
dcterms:license "https://creativecommons.org/licenses/by/1.0" ;
dcterms:modified "2021-08-13"^^xsd:date ;
dcterms:title "Stone Renovation Measures Ontology"@en ;
vann:preferredNamespacePrefix "srmo" ;
vann:preferredNamespaceUri "https://w3id.org/srmo#" ;
owl:versionInfo "0.1" .

#################################################################
#    Object Properties
#################################################################

###  https://w3id.org/srmo#recommendedRepairTask
srmo:recommendedRepairTask rdf:type owl:ObjectProperty ;
                           rdfs:domain sco:StoneComponent ;
                           rdfs:range srmo:StoneRepairTask ;
                           rdfs:label "Empfohlene Sanierungsmaßnahme"@de ,
                                      "Recommended repair task"@en .

#################################################################
#    Classes
#################################################################


###  https://w3id.org/srmo#Anchoring
srmo:Anchoring rdf:type owl:Class ;
               rdfs:subClassOf srmo:StructuralConstructiveMeasure ;
               rdfs:label "Anchoring"@en ,
                          "Verankern"@de .


###  https://w3id.org/srmo#BiocidalTreatment
srmo:BiocidalTreatment rdf:type owl:Class ;
                       rdfs:subClassOf srmo:ChemicalCleaning ;
                       rdfs:comment "Stone cleaning measure that involves the use of biocides in order to deter, render harmless or destroy harmful organisms."@en ;
                       rdfs:label "Biocidal Treatment"@en ,
                                  "Biozide Behandlung"@de .


###  https://w3id.org/srmo#Bracing
srmo:Bracing rdf:type owl:Class ;
             rdfs:subClassOf srmo:StructuralConstructiveMeasure ;
             rdfs:label "Bracing"@en ,
                        "Verklammern"@de .


###  https://w3id.org/srmo#ChemicalCleaning
srmo:ChemicalCleaning rdf:type owl:Class ;
                      rdfs:subClassOf srmo:Cleaning ;
                      rdfs:comment "Stone Cleaning measure that involves the use of chemical substances."@en ;
                      rdfs:label "Chemical Cleaning"@en ,
                                 "Chemische Abnahme"@de .


###  https://w3id.org/srmo#Cleaning
srmo:Cleaning rdf:type owl:Class ;
              rdfs:subClassOf srmo:StoneRepairTask ;
              rdfs:comment "Renovation measure that aims for cleaning a stones surface from impuritites and contamination."@en ;
              rdfs:label "Cleaning"@en ,
                         "Reinigung"@de .


###  https://w3id.org/srmo#CrackFilling
srmo:CrackFilling rdf:type owl:Class ;
                  rdfs:subClassOf srmo:NonStructuralConstructiveMeasure ;
                  rdfs:comment "Measure that fills the crack of a stone. Usually does not fix the damage source, thus a reoccurence of the same damage is possible."@en ;
                  rdfs:label "Crack Filling"@en ,
                             "Rissverfüllung"@de .


###  https://w3id.org/srmo#DryCleaning
srmo:DryCleaning rdf:type owl:Class ;
                 rdfs:subClassOf srmo:MechanicalCleaning ;
                 rdfs:comment "Cleaning measure that does not involve the use of wet substances, such as water to clean the stone."@en ;
                 rdfs:label "Dry Cleaning"@en ,
                            "Trockenreinigung"@de .


###  https://w3id.org/srmo#Flaming
srmo:Flaming rdf:type owl:Class ;
             rdfs:subClassOf srmo:ChemicalCleaning ;
             rdfs:comment "Application of high temperature to the surface of stones to remove organic material through burning."@en ;
             rdfs:label "Abflammen"@de ,
                        "Flame"@en .


###  https://w3id.org/srmo#Maintenance_measure
srmo:Maintenance_measure rdf:type owl:Class ;
                         rdfs:subClassOf srmo:PreventiveMeasure ;
                         rdfs:comment "Inspection and repair of minor defects or damages on the stone to prevent their aggravation."@en ;
                         rdfs:label "Maintenance Measure"@en ,
                                    "Wartungsarbeiten"@de .


###  https://w3id.org/srmo#MechanicalCleaning
srmo:MechanicalCleaning rdf:type owl:Class ;
                        rdfs:subClassOf srmo:Cleaning ;
                        rdfs:comment "Stone Cleaning measure that involves the use of mechanic-based procedures to remove inpurities and contamination."@en ;
                        rdfs:label "Mechanical Cleaning"@en ,
                                   "Mechanische Abnahme"@de .


###  https://w3id.org/srmo#Needling
srmo:Needling rdf:type owl:Class ;
              rdfs:subClassOf srmo:StructuralConstructiveMeasure ;
              rdfs:label "Needling"@en ,
                         "Vernadeln"@de .


###  https://w3id.org/srmo#NonStructuralConstructiveMeasure
srmo:NonStructuralConstructiveMeasure rdf:type owl:Class ;
                                      rdfs:subClassOf srmo:SecuringMeasure ;
                                      rdfs:comment "Constructive measure that does not significantly restore the structural capacity of the stone."@en ;
                                      rdfs:label "Nicht Statisch-Konstruktive Maßnahmen"@de ,
                                                 "Non-structural constructive measures"@en .


###  https://w3id.org/srmo#Plastering
srmo:Plastering rdf:type owl:Class ;
                rdfs:subClassOf srmo:PreventiveMeasure ;
                rdfs:comment "Applies or renews the plaster of the building element."@en ;
                rdfs:label "Neuputz"@de ,
                           "Plastering"@en .


###  https://w3id.org/srmo#Pressing
srmo:Pressing rdf:type owl:Class ;
              rdfs:subClassOf srmo:StructuralConstructiveMeasure ;
              rdfs:label "Pressing"@en ,
                         "Verpressen"@de .


###  https://w3id.org/srmo#PreventiveBiocidalTreatment
srmo:PreventiveBiocidalTreatment rdf:type owl:Class ;
                                 rdfs:subClassOf srmo:PreventiveMeasure ;
                                 rdfs:comment "Measure that involves the use of biocides in order to prevent the settlement of organic material on the stone."@en ;
                                 rdfs:label "Preventive Biocidal Treatment"@en ,
                                            "Präventive Biozide Behandlung"@de .


###  https://w3id.org/srmo#PreventiveMeasure
srmo:PreventiveMeasure rdf:type owl:Class ;
                       rdfs:subClassOf srmo:StoneRepairTask ;
                       rdfs:comment "Measure or steps taken for preventing the stone deterioration preemptively before damages or defects occur."@en ;
                       rdfs:label "Preventive Measure"@en ,
                                  "Präventive Maßnahme"@de .


###  https://w3id.org/srmo#SecuringMeasure
srmo:SecuringMeasure rdf:type owl:Class ;
                     rdfs:subClassOf srmo:StoneRepairTask ;
                     rdfs:comment "Measure, which secures the stone and prevent further degradation of its material due to structural effects."@en ;
                     rdfs:label "Securing Measure"@en ,
                                "Sicherungsmaßnahme"@de .


###  https://w3id.org/srmo#StoneComplement
srmo:StoneComplement rdf:type owl:Class ;
                     rdfs:subClassOf srmo:StoneRepairTask ;
                     rdfs:comment "Measure in which missing parts of a stone are complemented."@en ;
                     rdfs:label "Steinergänzung"@de ,
                                "Stone Complement"@en .


###  https://w3id.org/srmo#StoneRepairTask
srmo:StoneRepairTask rdf:type owl:Class ;
                     rdfs:subClassOf cto:RepairTask ;
                     rdfs:comment "A repair task that specifically aims for the renovation of deteriorated stone structures."@en ;
                     rdfs:label "Steinsanierungsmaßnahme"@de ,
                                "Stone repair task"@en .


###  https://w3id.org/srmo#StoneReplacement
srmo:StoneReplacement rdf:type owl:Class ;
                      rdfs:subClassOf srmo:StoneRepairTask ;
                      rdfs:comment "Measure in which a stone is completely replaced with a new stone."@en ;
                      rdfs:label "Steinaustausch"@de ,
                                 "Stone Replacement"@en .


###  https://w3id.org/srmo#StructuralConstructiveMeasure
srmo:StructuralConstructiveMeasure rdf:type owl:Class ;
                                   rdfs:subClassOf srmo:SecuringMeasure ;
                                   rdfs:comment "Constructive measure that does restore the structural capacity of the stone and in consequence of the building element in which it is aggregated."@en ;
                                   rdfs:label "Statisch-Konstruktive Maßnahme"@de ,
                                              "Structural constructive measure"@en .


###  https://w3id.org/srmo#WetCleaning
srmo:WetCleaning rdf:type owl:Class ;
                 rdfs:subClassOf srmo:MechanicalCleaning ;
                 rdfs:comment "Cleaning measure that does involve the use of wet substances, such as water to clean the stone."@en ;
                 rdfs:label "Nassreinigung"@de ,
                            "Wet Cleaning"@en .
